rustexamples/test/borrow_test/25.rs
@@ -1,0 +1,36 @@
+struct list<'a>;
+
+enum list_node<'a>;
+
+enum list_node<'a> {
+    None,
+    Some(&'a mut list<'a>)
+}
+
+struct list<'a> {
+    value: i32,
+    next: list_node<'a>
+}
+
+fn sum<'a>(l: &'a mut list<'a>) -> i32 {
+    let result: i32 = 0;
+    result = result + (*l).value;
+    loop {
+        match (*l).next {
+            list_node::Some(ref mut r) => {
+                l = &mut **r;
+            }
+            list_node::None => {
+                return result;
+            }
+        }
+    }
+    return result;
+}
+
+fn main(){
+    let l0: list = list {value: 1, next: list_node::None(())};
+    let l1: list = list {value: 2, next: list_node::Some(&mut l0)};
+    let l2: list = list {value: 3, next: list_node::Some(&mut l1)};
+    printf("Sum of list is %d", sum(&mut l2));
+}
